DLean/USubst/Semantics.lean
@@ -702,30 +702,32 @@ decreasing_by
 
 lemma ode_mapM_assignables_eq
   {σ : Subst}
+  {U : FCSet Assignable}
   {system : OdeSystem}
   {ssystem : OdeSystem}
-  (h : system.mapM (fun x => do return ODE.mk x.var (← Term.applySubst σ ∅ x.term))
+  (h : system.mapM (fun x => do return ODE.mk x.var (← Term.applySubst σ U x.term))
        = some ssystem)
   : OdeSystem.assignables ssystem = OdeSystem.assignables system := by
   unfold OdeSystem.assignables at *;
   induction system generalizing ssystem <;> simp_all +decide [ List.mapM_cons ];
-  cases h' : Term.applySubst σ ∅ ‹ODE›.term <;> simp_all +decide [ Option.bind_eq_some_iff ];
+  cases h' : Term.applySubst σ U ‹ODE›.term <;> simp_all +decide [ Option.bind_eq_some_iff ];
   aesop
 
 lemma ode_evolution_formula_applySubst
   {σ : Subst}
+  {U : FCSet Assignable}
   {system ssystem : OdeSystem}
   {Ψ Ψ' : Formula}
-  : Formula.applySubst σ Ψ = some Ψ'
-  → system.mapM (fun x => do return ODE.mk x.var (← Term.applySubst σ ∅ x.term)) = some ssystem
-  → Formula.applySubst σ (odeEvolutionFormula system Ψ)
+  : Formula.applySubst σ U Ψ = some Ψ'
+  → system.mapM (fun x => do return ODE.mk x.var (← Term.applySubst σ U x.term)) = some ssystem
+  → Formula.applySubst σ U (odeEvolutionFormula system Ψ)
   = some (odeEvolutionFormula ssystem Ψ') := by
 
   intros h₁ h₂
   induction system generalizing ssystem Ψ Ψ' with
     | nil => simp_all[odeEvolutionFormula]
     | cons head tail ih =>
-      cases _ : Term.applySubst σ ∅ head.term
+      cases _ : Term.applySubst σ U head.term
       . simp_all
       .
         simp_all[Option.bind_eq_some_iff]
@@ -758,6 +760,77 @@ lemma ode_evolution_formula_admissible
     unfold Subst.admissible; aesop;
   exact h_foldr system hterms
 
+lemma Program.boundVars_applySubst_subset
+  (σ : Subst)
+  (U : FCSet Assignable)
+  (α α' : Program) :
+  Program.applySubst σ U α = α' → α'.boundVars ⊆ α.boundVars := by
+  intro h
+  match α with
+  | .const a =>
+    simp[Program.boundVars]
+  | .test _ =>
+    simp[Program.applySubst, Option.bind] at h
+    split at h
+    . contradiction
+    simp at h
+    rw[←h]
+    simp[Program.boundVars]
+  | .assign _ _ =>
+    simp[Program.applySubst, Option.bind] at h
+    split at h
+    . contradiction
+    simp at h
+    rw[←h]
+    simp[Program.boundVars]
+  | .random _ =>
+    simp[Program.applySubst] at h
+    rw[←h]
+  | .choice β γ
+  | .seq β γ =>
+    simp[Program.applySubst, Option.bind] at h
+    split at h
+    . contradiction
+    simp only at h
+    split at h
+    . contradiction
+    simp at h
+    next β' hβ _ _ γ' hγ =>
+      apply Program.boundVars_applySubst_subset at hγ
+      apply Program.boundVars_applySubst_subset at hβ
+      grind only [= Set.subset_def, boundVars, = Set.mem_union]
+  | .loop β =>
+    simp[Program.applySubst, Option.bind] at h
+    split at h
+    . contradiction
+    simp only at h
+    split at h
+    . contradiction
+    simp at h
+    next β' hβ =>
+      apply Program.boundVars_applySubst_subset at hβ
+      grind only [boundVars]
+  | .ode sys _ =>
+    simp[Program.applySubst, Option.bind] at h
+    split at h
+    . contradiction
+    simp only at h
+    split at h
+    . contradiction
+    simp at h
+    next sys' hsys =>
+      have hassign : OdeSystem.assignables sys' = OdeSystem.assignables sys :=
+          ode_mapM_assignables_eq (show _ = some sys' from ‹_›)
+      grind only [boundVars, = Set.subset_def]
+
+lemma Program.boundVars'_applySubst_subset
+  (σ : Subst)
+  (U : FCSet Assignable)
+  (α α' : Program) :
+  Program.applySubst σ U α = α' → α'.boundVars'.toSet ⊆ α.boundVars'.toSet := by
+  rw[←Program.bound_vars_decidable α, ←Program.bound_vars_decidable α']
+  apply Program.boundVars_applySubst_subset
+
 set_option maxHeartbeats 0 in
 /- Good things take time (dunno if that is one of them) --/
 
@@ -765,11 +838,13 @@ mutual
 
 theorem Subst.preserve_semantics.formula
   (σ : Subst)
+  (U : FCSet Assignable)
   (i : Interpretation)
-  (v : State)
+  (v w : State)
+  (hvw : v.isEqExcept w U)
   (Φ Φ' : Formula)
-  (hs : Φ' = Formula.applySubst σ Φ)
-  : v ∈ Formula.denote i Φ' ↔ v ∈ Formula.denote (Subst.adjoint σ i v) Φ := by
+  (hs : Φ' = Formula.applySubst σ U Φ)
+  : v ∈ Formula.denote i Φ' ↔ v ∈ Formula.denote (Subst.adjoint σ i w) Φ := by
     match Φ with
       | .True
       | .False =>
@@ -783,8 +858,8 @@ theorem Subst.preserve_semantics.formula
         split at hs
         . contradiction
         simp_all[Formula.denote]
-        have := Subst.preserve_semantics.term σ ∅ i v _ (Set.eqOn_refl _ _) t₁
-        have := Subst.preserve_semantics.term σ ∅ i v _ (Set.eqOn_refl _ _) t₂
+        have := Subst.preserve_semantics.term σ U i v w hvw t₁
+        have := Subst.preserve_semantics.term σ U i v w hvw t₂
         grind
       | .not Φ =>
         simp_all[Formula.denote, Formula.applySubst, Option.bind]
@@ -792,7 +867,7 @@ theorem Subst.preserve_semantics.formula
         . contradiction
         simp_all
         rename Formula => Φ'
-        have := Subst.preserve_semantics.formula σ i v Φ Φ'
+        have := Subst.preserve_semantics.formula σ U i v w hvw Φ Φ'
         simp_all[Formula.denote]
       | .and Φ₁ Φ₂ =>
         simp_all[Formula.denote, Formula.applySubst, Option.bind]
@@ -803,69 +878,46 @@ theorem Subst.preserve_semantics.formula
         . contradiction
         simp_all
         next Φ₁' _ _ _ Φ₂' _ =>
-        have := Subst.preserve_semantics.formula σ i v Φ₁ Φ₁'
-        have := Subst.preserve_semantics.formula σ i v Φ₂ Φ₂'
+        have := Subst.preserve_semantics.formula σ U i v w hvw Φ₁ Φ₁'
+        have := Subst.preserve_semantics.formula σ U i v w hvw Φ₂ Φ₂'
         simp_all[Formula.denote]
       | .forall x Φ =>
         simp_all[Formula.denote, Formula.applySubst, Option.bind]
         split at hs
         . contradiction
         simp_all
-        split at hs
-        . contradiction
         rename Formula => Φ'
         simp_all[Formula.denote]
         apply Iff.intro
         .
           intros h r
-          have := (Subst.preserve_semantics.formula σ i (v.update x r) Φ Φ' (by grind)).mp (h r)
-          have := Subst.admissible_adjoint.formula (U := {.var x}) (Φ := Φ) (i := i) (σ := σ)
-                                                   (v := v) (w := v.update x r)
-                                                   (by simp_all[Subst.admissible])
-                                                   (by simp_all[State.isEqOn, Set.EqOn])
-          rw[this]
-          grind
+          have hvw' : (v.update x r).isEqExcept w ({.var x} ∪ U).toSet := by grind[Set.EqOn, State.isEqExcept]
+          apply (Subst.preserve_semantics.formula σ ({.var x} ∪ U) i (v.update x r) w hvw' Φ Φ' (by grind)).mp (h r)
+
         .
           intros h r
-          have := Subst.admissible_adjoint.formula (U := {.var x}) (Φ := Φ) (i := i) (σ := σ)
-                                                   (v := v) (w := v.update x r)
-                                                   (by simp_all[Subst.admissible])
-                                                   (by simp_all[State.isEqOn, Set.EqOn])
-          rw[this] at h
-          have := (Subst.preserve_semantics.formula σ i (v.update x r) Φ Φ' (by grind)).mpr (h r)
-          grind
+          have hvw' : (v.update x r).isEqExcept w ({.var x} ∪ U).toSet := by grind[Set.EqOn, State.isEqExcept]
+          apply (Subst.preserve_semantics.formula σ ({.var x} ∪ U) i (v.update x r) w hvw' Φ Φ' (by grind)).mpr (h r)
       | .exists x Φ =>
         simp_all[Formula.denote, Formula.applySubst, Option.bind]
         split at hs
         . contradiction
         simp_all
-        split at hs
-        . contradiction
         rename Formula => Φ'
         simp_all[Formula.denote]
         apply Iff.intro
         .
-          intros h
-          obtain ⟨r, hr⟩ := h
+          intro ⟨r, hr⟩
           apply Exists.intro r
 
-          have := Subst.preserve_semantics.formula σ i (v.update x r) Φ Φ' (by grind)
-          have := Subst.admissible_adjoint.formula (U := {.var x}) (Φ := Φ) (i := i) (σ := σ)
-                                                   (v := v) (w := v.update x r)
-                                                   (by simp_all[Subst.admissible])
-                                                   (by simp_all[State.isEqOn, Set.EqOn])
-          grind
+          have hvw' : (v.update x r).isEqExcept w ({.var x} ∪ U).toSet := by grind[Set.EqOn, State.isEqExcept]
+          apply (Subst.preserve_semantics.formula σ ({.var x} ∪ U) i (v.update x r) w hvw' Φ Φ' (by grind)).mp hr
         .
-          intros h
-          obtain ⟨r, hr⟩ := h
+          intro ⟨r, hr⟩
           apply Exists.intro r
 
-          have := Subst.preserve_semantics.formula σ i (v.update x r) Φ Φ' (by grind)
-          have := Subst.admissible_adjoint.formula (U := {.var x}) (Φ := Φ) (i := i) (σ := σ)
-                                                   (v := v) (w := v.update x r)
-                                                   (by simp_all[Subst.admissible])
-                                                   (by simp_all[State.isEqOn, Set.EqOn])
-          grind
+          have hvw' : (v.update x r).isEqExcept w ({.var x} ∪ U).toSet := by grind[Set.EqOn, State.isEqExcept]
+          apply (Subst.preserve_semantics.formula σ ({.var x} ∪ U) i (v.update x r) w hvw' Φ Φ' (by grind)).mpr hr
       | .box α Φ =>
         simp_all[Formula.denote, Formula.applySubst, Option.bind]
         split at hs
@@ -874,24 +926,22 @@ theorem Subst.preserve_semantics.formula
         split at hs
         . contradiction
         simp_all
-        split at hs
-        . contradiction
         rename Program => α'
         rename Formula => Φ'
         simp_all[Formula.denote]
+        set V := α'.boundVars' ∪ U
         apply Iff.intro
         all_goals
-        -- guard <| σ.admissible σα.boundVars' Φ.signature
-        intros h₁ w h₂
-        have := Program.bound_effect h₂
-        have := Subst.preserve_semantics.program σ i v w α α'
-        have := Subst.admissible_adjoint.formula (U := α'.boundVars')
-                                                 (Φ := Φ) (i := i)
-                                                 (σ := σ) (v := v) (w := w)
-                                                 (by simp_all[Subst.admissible])
-                                                 (by grind[Program.bound_effect'])
-        have := Subst.preserve_semantics.formula σ i w Φ Φ'
-        grind
+        intros h₁ w' h₂
+        have := Subst.preserve_semantics.program σ U i v w w' hvw α α'
+        simp_all only [iff_true, forall_const]
+        have := Program.bound_effect this
+        rw[Program.bound_vars_decidable α'] at this
+        have hww' : w'.isEqExcept w V.toSet := by
+          grind only [FCSet.to_set_union, State.isEqExcept, Set.EqOn, = Set.mem_compl_iff,
+            = Set.mem_union]
+        have := Subst.preserve_semantics.formula σ V i w' w hww' Φ Φ'
+        grind only
       | .diamond α Φ =>
         simp_all[Formula.denote, Formula.applySubst, Option.bind]
         split at hs
@@ -900,24 +950,23 @@ theorem Subst.preserve_semantics.formula
         split at hs
         . contradiction
         simp_all
-        split at hs
-        . contradiction
         rename Program => α'
         rename Formula => Φ'
         simp_all[Formula.denote]
+        set V := α'.boundVars' ∪ U
         apply Iff.intro
         all_goals
-        intros h
-        obtain ⟨w, hw⟩ := h
-        apply Exists.intro w
-        have := Subst.preserve_semantics.program σ i v w α α'
-        have := Subst.admissible_adjoint.formula (U := α'.boundVars')
-                                               (Φ := Φ) (i := i)
-                                               (σ := σ) (v := v) (w := w)
-                                               (by simp_all[Subst.admissible])
-                                               (by grind[Program.bound_effect'])
-        have := Subst.preserve_semantics.formula σ i w Φ Φ'
-        grind
+        intro ⟨w', hw⟩
+        apply Exists.intro w'
+        have := Subst.preserve_semantics.program σ U i v w w' hvw α α'
+        simp_all only [iff_true, forall_const, and_true]
+        have := Program.bound_effect this
+        rw[Program.bound_vars_decidable α'] at this
+        have hww' : w'.isEqExcept w V.toSet := by
+          grind only [FCSet.to_set_union, State.isEqExcept, Set.EqOn, = Set.mem_compl_iff,
+            = Set.mem_union]
+        have := Subst.preserve_semantics.formula σ V i w' w hww' Φ Φ'
+        grind only
       | .ref α β =>
         simp_all[Formula.denote, Formula.applySubst, Option.bind]
         split at hs
@@ -929,36 +978,47 @@ theorem Subst.preserve_semantics.formula
         next _ _ α' _ _ _ β' _ =>
         apply Iff.intro
         all_goals
-        intros h₁ w h₂
-        have := Subst.preserve_semantics.program σ i v w α α'
-        have := Subst.preserve_semantics.program σ i v w β β'
+        intros h₁ w' h₂
+        have := Subst.preserve_semantics.program σ U i v w w' hvw α α'
+        have := Subst.preserve_semantics.program σ U i v w w' hvw β β'
         grind
       | .applyPred p args =>
-        simp_all[Formula.denote, Formula.applySubst, Option.bind]
+        simp[Formula.applySubst, Option.bind] at hs
         split at hs
         . contradiction
-        simp_all
+        simp only at hs
 
         next _ args' _ =>
-        have : (fun (x : Fin p.arity) => Term.denote (σ.adjoint i v) v args.toVector[↑(x : ℕ)])
+        have : (fun (x : Fin p.arity) => Term.denote (σ.adjoint i w) v args.toVector[↑(x : ℕ)])
              = (fun (x : Fin p.arity) => Term.denote i v args'.toVector[↑x]) := by
                   funext x
                   apply Eq.symm
-                  apply Subst.preserve_semantics.term _ ∅ _ _ _ (Set.eqOn_refl _ _)
+                  apply Subst.preserve_semantics.term _ U _ _ _ hvw
                   apply Eq.symm
                   apply Subst.apply_subst_term_vector_to_term
                   assumption
 
         split at hs
-        .
+        . split at hs
+          . contradiction
+          simp_all
           -- we do apply the subst
-          apply Subst.preserve_semantics.formula (σ := args'.toSubst) (v := v) (i := i) at hs
-          rw[hs]
-          rw[subst_adjoint_of_term_vector_to_subst]
-          simp_all[Subst.adjoint]
+          apply Subst.preserve_semantics.formula args'.toSubst ∅ i v v at hs
+          .
+            rw[hs]
+            rw[subst_adjoint_of_term_vector_to_subst]
+            simp[Formula.denote, adjoint]
+            rw[this]
+            apply Iff.intro
+            all_goals
+            apply Formula.coincidence
+            simp_all[State.isEqExcept, ←Set.disjoint_iff_inter_eq_empty]
+            grind only [Formula.free_vars_decidable, = Set.disjoint_left, Set.EqOn, = Set.mem_compl_iff]
+          .
+            simp_all only [State.isEqExcept, FCSet.to_set_empty, Set.compl_empty, Set.eqOn_univ]
         .
           -- we dont apply the subst
-          have := @Subst.adjoint_noeffect_nomem_pred i v p σ (by assumption)
+          have := @Subst.adjoint_noeffect_nomem_pred i w p σ (by assumption)
           simp_all[Formula.denote, Subst.adjoint]
 termination_by (σ.size, Φ.size)
 decreasing_by
@@ -977,11 +1037,13 @@ decreasing_by
 
 theorem Subst.preserve_semantics.program
   (σ : Subst)
+  (U : FCSet Assignable)
   (i : Interpretation)
-  (v w : State)
+  (v v' w : State)
+  (hvv' : v.isEqExcept v' U)
   (α α' : Program)
-  (hs : α' = Program.applySubst σ α)
-  : ⟨v, w⟩ ∈ Program.denote i α' ↔ ⟨v, w⟩ ∈ Program.denote (Subst.adjoint σ i v) α := by
+  (hs : α' = Program.applySubst σ U α)
+  : ⟨v, w⟩ ∈ Program.denote i α' ↔ ⟨v, w⟩ ∈ Program.denote (Subst.adjoint σ i v') α := by
     match α with
       | .const a =>
         simp_all[Program.denote, Program.applySubst, Subst.adjoint]
@@ -991,7 +1053,7 @@ theorem Subst.preserve_semantics.program
         . contradiction
         rename Term => t'
         simp_all[Program.denote]
-        have := Subst.preserve_semantics.term σ ∅ i v _ (Set.eqOn_refl _ _) t t'
+        have := Subst.preserve_semantics.term σ U i v _ hvv' t t'
         grind
       | .random x =>
         simp[Program.applySubst] at hs
@@ -1003,7 +1065,7 @@ theorem Subst.preserve_semantics.program
         . contradiction
         rename Formula => Φ'
         simp_all[Program.denote]
-        have := Subst.preserve_semantics.formula σ i v Φ Φ'
+        have := Subst.preserve_semantics.formula σ U i v _ hvv' Φ Φ'
         grind
       | .choice α β =>
         simp_all[Program.denote, Program.applySubst, Option.bind]
@@ -1014,118 +1076,78 @@ theorem Subst.preserve_semantics.program
         . contradiction
         simp_all[Program.denote]
         next _ _ _ α' _ _ _ β' _ =>
-        have := Subst.preserve_semantics.program σ i v w α α'
-        have := Subst.preserve_semantics.program σ i v w β β'
+        have := Subst.preserve_semantics.program σ U i v _ w hvv' α α'
+        have := Subst.preserve_semantics.program σ U i v _ w hvv' β β'
         grind
       | .seq α β =>
-        simp_all[Program.denote, Program.applySubst, Option.bind]
+        simp[Program.applySubst, Option.bind] at hs
         split at hs
         . contradiction
-        simp_all
-        split at hs
-        . contradiction
+        simp only at hs
         split at hs
         . contradiction
         simp_all[Program.denote]
-        next α' _ _ _ _ _ _ β' _ _  =>
+        next α' _ _ _ β' _  =>
+        set V := α'.boundVars' ∪ U
         apply Iff.intro
-        .
-          intros h
-          obtain ⟨w', hw'⟩ := h
+        all_goals
+          intro ⟨w', hw'⟩
           apply Exists.intro w'
-          and_intros
-          .
-            have := Subst.preserve_semantics.program σ i v w' α α'
-            grind
-          .
-            have := Subst.preserve_semantics.program σ i w' w β β'
-            have := Subst.admissible_adjoint.program (U := α'.boundVars')
-                                                     (α := β) (i := i)
-                                                     (σ := σ) (v := v) (w := w')
-                                                     (by simp_all[Subst.admissible])
-                                                     (by grind[Program.bound_effect'])
-
-            grind
-        .
-          intros h
-          obtain ⟨w', hw'⟩ := h
-          apply Exists.intro w'
-          and_intros
-          .
-            have := Subst.preserve_semantics.program σ i v w' α α'
-            grind
-          .
-            have := Subst.preserve_semantics.program σ i v w' α α'
-            have := Subst.preserve_semantics.program σ i w' w β β'
-            have := Subst.admissible_adjoint.program (U := α'.boundVars')
-                                                     (α := β) (i := i)
-                                                     (σ := σ) (v := v) (w := w')
-                                                     (by simp_all[Subst.admissible])
-                                                     (by grind[Program.bound_effect'])
-
-            grind
+          have := Subst.preserve_semantics.program σ U i v _ w' hvv' α α'
+          simp_all only [iff_true, forall_const, true_and]
+          have := Program.bound_effect this
+          rw[Program.bound_vars_decidable α'] at this
+          have hw'v' : w'.isEqExcept v' V.toSet := by
+            grind only [FCSet.to_set_union, State.isEqExcept, Set.EqOn, = Set.mem_compl_iff,
+              = Set.mem_union]
+          have := Subst.preserve_semantics.program σ V i w' _ w hw'v' β β'
+          grind only
       | .loop α =>
-        simp_all[Program.denote, Program.applySubst, Option.bind]
+        simp[Program.applySubst, Option.bind] at hs
         split at hs
         . contradiction
-        simp_all
-        split at hs
-        . contradiction
+        -- first pass to get bound variables
+        simp at hs
         rename Program => α'
+        have := Subst.preserve_semantics.program σ U i v _ w hvv' α α'
+        set V := α'.boundVars' ∪ U
+        split at hs
+        . contradiction
+        rename Program => α''
+        have : α'' = α' := by grind only [Program.applySubst_unique]
+
         simp_all[Program.denote]
-        have := Subst.preserve_semantics.program σ i v w α α'
         apply Iff.intro
-        .
+        all_goals
           intros h
           induction h with
             | rfl => grind[LoopClosure]
-            | trans v w h₁ h₂ ih =>
-                have := ih (by apply Subst.preserve_semantics.program)
-                apply LoopClosure.trans (v := v)
+            | trans v₂ w h₁ h₂ ih =>
+                have := ih (by apply Subst.preserve_semantics.program _ _ _ _ _ _ hvv'; simp_all only)
+                apply LoopClosure.trans (v := v₂)
                 . grind
                 .
-                  next u _ _ _ _ _ _ _ _ _ _ _ =>
-                  have := (Subst.preserve_semantics.program σ i v w α α' (by grind)).mp h₂
-                  have := Subst.admissible_adjoint.program (U := α'.boundVars') (α := α) (i := i)
-                                                           (σ := σ) (v := u) (w := v)
-                            (by simp_all[Subst.admissible])
-                            (by grind)
-
-                  simp_all[Membership.mem, Set.Mem]
-        .
-          intros h
-          induction h with
-            | rfl => grind[LoopClosure]
-            | trans v w h₁ h₂ ih =>
-              have := ih (by apply Subst.preserve_semantics.program)
-              apply LoopClosure.trans (v := v)
-              . grind
-              .
-                next u _ _ _ _ _ _ _ _ _ _ _ =>
-                have := Subst.admissible_adjoint.program (U := α'.boundVars') (α := α) (i := i)
-                                                         (σ := σ) (v := u) (w := v)
-                         (by simp_all[Subst.admissible])
-                         (by grind)
-
-                have := (Subst.preserve_semantics.program σ i v w α α' (by grind)).mpr
-                  (by rw[← this] ; exact h₂)
-
-                simp_all[Membership.mem, Set.Mem]
+                  have := @Program.bound_effect α'.loop v v₂ i
+                  rw[Program.bound_vars_decidable α'.loop] at this
+                  simp_all[Program.denote, Program.boundVars']
+                  have hv₂v' : v₂.isEqExcept v' V.toSet := by
+                    grind only [!FCSet.to_set_union, State.isEqExcept, Set.EqOn,
+                      = Set.mem_compl_iff, = Set.mem_union]
+                  have := Subst.preserve_semantics.program σ V i v₂ v' w hv₂v' α α'
+                  simp_all[V,Membership.mem, Set.Mem]
       | .ode system Ψ =>
         simp[Program.applySubst, Option.bind] at hs
         split at hs
         . contradiction
-        simp_all
+        simp only at hs
         split at hs
         . contradiction
         simp_all
-        split at hs
-        . contradiction
-        simp_all
-        split at hs
-        . contradiction
         rename List ODE => ssystem
         rename Formula => Ψ'
+        let vars := (system.map ODE.var).toFinset
+        let vars' := vars.map Assignable.diff_emb
+        set V := (.Finite (vars ∪ vars')) ∪ U
         simp_all[Program.denote]
 
         have hassign : OdeSystem.assignables ssystem = OdeSystem.assignables system :=
@@ -1133,7 +1155,8 @@ theorem Subst.preserve_semantics.program
 
         rw[hassign]
         apply Iff.intro
-        . rintro ⟨r, hr, φ, heq0, heqr, hflow⟩
+        all_goals
+          rintro ⟨r, hr, φ, heq0, heqr, hflow⟩
           apply Exists.intro r
           and_intros
           . grind
@@ -1149,66 +1172,17 @@ theorem Subst.preserve_semantics.program
                 have := hflow ζ h₁ h₂
 
                 have := ode_evolution_formula_applySubst
-                          (σ := σ) (system := system) (ssystem := ssystem)
+                          (σ := σ) (U := V) (system := system) (ssystem := ssystem)
                           (Ψ := Ψ) (Ψ' := Ψ') (by grind) (by grind)
 
-                have := Subst.preserve_semantics.formula σ i (φ ζ)
+                have hφv' : (φ ζ).isEqExcept v' V.toSet := by
+                  specialize hflow ζ h₁ h₂
+                  clear * - hvv' heq0 hflow
+                  grind[State.isEqExcept, Set.EqOn, OdeSystem.assignables]
+                have := Subst.preserve_semantics.formula σ V i (φ ζ) v' hφv'
                           (odeEvolutionFormula system Ψ)
                           (odeEvolutionFormula ssystem Ψ') (by grind)
-
-                have := this.mp (by grind)
-
-                have := ode_evolution_formula_admissible σ system Ψ
-                          (.Finite (system.assignables ∪ system.assignables.map Assignable.diff_emb))
-                          (by simp_all[Subst.admissible, OdeSystem.assignables])
-                          (by simp_all[Subst.admissible, OdeSystem.assignables])
-
-                have := Subst.admissible_adjoint.formula
-                          (v := v) (w := φ ζ) (σ := σ)
-                          (i := i) (Φ := odeEvolutionFormula system Ψ)
-                          (U := .Finite (system.assignables ∪ system.assignables.map Assignable.diff_emb))
-                          (by simp_all [Subst.admissible])
-                          (by simp_all[State.isEqOn, State.isEqExcept, Set.EqOn])
-
-                grind
-              . grind
-              . grind
-        . rintro ⟨r, hr, φ, heq0, heqr, hflow⟩
-          apply Exists.intro r
-          and_intros
-          . grind
-          .
-            apply Exists.intro φ
-            and_intros
-            . grind
-            . grind
-            .
-              intros ζ h₁ h₂
-              and_intros
-              .
-                have := hflow ζ h₁ h₂
-
-                have := ode_evolution_formula_applySubst
-                          (σ := σ) (system := system) (ssystem := ssystem)
-                          (Ψ := Ψ) (Ψ' := Ψ') (by grind) (by grind)
-
-                have := Subst.preserve_semantics.formula σ i (φ ζ)
-                          (odeEvolutionFormula system Ψ)
-                          (odeEvolutionFormula ssystem Ψ') (by grind)
-
-                have := ode_evolution_formula_admissible σ system Ψ
-                          (.Finite (system.assignables ∪ system.assignables.map Assignable.diff_emb))
-                          (by simp_all[Subst.admissible, OdeSystem.assignables])
-                          (by simp_all[Subst.admissible, OdeSystem.assignables])
-
-                have := Subst.admissible_adjoint.formula
-                          (v := v) (w := φ ζ) (σ := σ)
-                          (i := i) (Φ := odeEvolutionFormula system Ψ)
-                          (U := .Finite (system.assignables ∪ system.assignables.map Assignable.diff_emb))
-                          (by simp_all [Subst.admissible])
-                          (by simp_all [State.isEqOn, State.isEqExcept, Set.EqOn])
-
-                grind
+                grind only
               . grind
               . grind
 termination_by (σ.size, α.size)
@@ -1220,35 +1194,30 @@ end
 
 -- Uniform Substitution for Differential Dynamic Logic is sound!
 theorem US {σ : Subst} {Φ Φ' : Formula}
-  : Formula.applySubst σ Φ = Φ'
+  : Formula.applySubst σ ∅ Φ = Φ'
   → (∀ (i : Interpretation) (v : State), v ∈ Formula.denote i Φ)
   → (∀ (i : Interpretation) (v : State), v ∈ Formula.denote i Φ') := by
   intros h₁ h₂ i v
   have := h₂ i v
-  have := Subst.preserve_semantics.formula σ i v Φ Φ' (by grind)
+  have := Subst.preserve_semantics.formula σ ∅ i v v (Set.eqOn_refl _ _) Φ Φ' (by grind)
   simp_all
 
 theorem US_rule {σ : Subst}
                 (premises : List (Formula × Formula))
                 (Ψ Ψ' : Formula)
-                (hp : ∀ Φ ∈ premises, Formula.applySubst σ Φ.1 = Φ.2)
-                (hΨ : Formula.applySubst σ Ψ = Ψ')
-                (hσ : Subst.freeVars σ .none = ∅)
+                (hp : ∀ Φ ∈ premises, Formula.applySubst σ .univ Φ.1 = Φ.2)
+                (hΨ : Formula.applySubst σ .univ Ψ = Ψ')
   : (∀ (i : Interpretation), (∀ (v : State) (Φ : Formula × Formula), Φ ∈ premises → v ∈ Formula.denote i Φ.1) → (∀ (v : State), v ∈ Formula.denote i Ψ))
   → (∀ (i : Interpretation), (∀ (v : State) (Φ : Formula × Formula), Φ ∈ premises → v ∈ Formula.denote i Φ.2) → (∀ (v : State), v ∈ Formula.denote i Ψ')) := by
   intros h₁ i h₂ v
 
-  have := by
-    apply h₁ (Subst.adjoint σ i v) (?_) v
+  have : ∀ (w : State), ∀ Φ ∈ premises, w ∈ Formula.denote (σ.adjoint i v) Φ.1:= by
     intros w Φ hp
-    have := Subst.preserve_semantics.formula σ i w Φ.1 Φ.2 (by grind)
-    have := Subst.freeVars_symbol_subset_none (σ := σ) (S := (Φ.1).signature)
-    have := Subst.admissible_adjoint.formula
-              (Φ := Φ.1) (i := i) (σ := σ)
-              (v := v) (w := w) (U := .univ)
-              (by simp_all [Subst.admissible])
-              (by simp_all)
-    grind
+    have := Subst.preserve_semantics.formula σ .univ i w v (by grind[State.isEqExcept, Set.EqOn]) Φ.1 Φ.2 (by grind only)
+    grind only
 
-  have := Subst.preserve_semantics.formula σ i v Ψ Ψ' (by grind)
-  grind
+  have : v ∈ Formula.denote (σ.adjoint i v) Ψ :=
+    h₁ (Subst.adjoint σ i v) this v
+
+  have := Subst.preserve_semantics.formula σ .univ i v v (Set.eqOn_refl _ _) Ψ Ψ' (by grind)
+  grind only
